Valaig/Transform/Unroll.lean
@@ -15,11 +15,11 @@ private def walker (old : Aig) : old.CachingForwardsWalker Aig Lit where
 
   step var aig cache valid size sm cm :=
     match _ : aig[var] with
-    | .false         => (aig, .false)
-    | .and rhs0 rhs1 => let (eq:=_) (aig, var) := aig.addAndRaw (cache.mapLit rhs0) (cache.mapLit rhs1)
-                        (aig, var)
-    | .input _       => let (eq:=_) (aig, idx) := aig.addInput; (aig, idx.getVar aig)
-    | .latch idx     => (aig, idx.getNext aig)
+    | .false       => (aig, .false)
+    | .and lhs rhs => let (eq:=_) (aig, var) := aig.addAndRaw (cache.mapLit lhs) (cache.mapLit rhs)
+                      (aig, var)
+    | .input _     => let (eq:=_) (aig, idx) := aig.addInput; (aig, idx.getVar aig)
+    | .latch idx   => (aig, idx.getNext aig)
 
   stepState := by intros; split <;> grind
   stepCache := by intros; split <;> grind
